\hypertarget{nonlinear-geometry}{%
\section{6 Nonlinear Geometry}\label{nonlinear-geometry}}

\[\delta v=\frac{\partial v}{\partial u} \delta u=\mathrm{a}_{g}(u) \delta u\]
\[\mathbf{k}_{m}=\mathbf{a}_{g}^{T}(\boldsymbol{u}) \frac{\partial \boldsymbol{q}}{\partial v} \mathbf{a}_{g}(\boldsymbol{u})\]

\[\begin{aligned}
\mathbf{k}_{e}=\frac{\partial \boldsymbol{p}}{\partial \boldsymbol{u}}=\frac{\partial\left[\mathbf{a}_{g}^{T}(\boldsymbol{u}) q\right]}{\partial \boldsymbol{u}} &=\mathbf{a}_{g}^{T}(\boldsymbol{u}) \frac{\partial q}{\partial \boldsymbol{u}}+\frac{\partial\left[\mathbf{a}_{g}^{T}(\boldsymbol{u})\right]}{\partial \boldsymbol{u}} q \\
&=\mathbf{a}_{g}^{T}(\boldsymbol{u}) \frac{\partial q}{\partial v} \frac{\partial v}{\partial \boldsymbol{u}}+\frac{\partial\left[\mathbf{a}_{g}^{T}(\boldsymbol{u})\right]}{\partial \boldsymbol{u}} q \\
&=\mathbf{a}_{g}^{T}(\boldsymbol{u}) \frac{\partial q}{\partial v} \mathbf{a}_{g}(\boldsymbol{u})+\frac{\partial\left[\mathbf{a}_{g}^{T}(\boldsymbol{u})\right]}{\partial \boldsymbol{u}} q \\
&=\mathbf{k}_{m} \quad+\mathbf{k}_{g}
\end{aligned}\]

\hypertarget{felippa}{%
\subsection{Felippa}\label{felippa}}

\[e=\mathbf{B}_{0} \mathbf{u}+\frac{1}{2} \mathbf{u}^{T} \mathbf{H} \mathbf{u}\]
\[\mathbf{K}=A_{0} L_{0} \mathbf{B}^{T} \frac{\partial s}{\partial \mathbf{u}}+A_{0} L_{0} s \frac{\partial \mathbf{B}^{T}}{\partial \mathbf{u}}=\mathbf{K}_{M}+\mathbf{K}_{G}\]
\[\mathbf{K}=\frac{\partial \mathbf{p}}{\partial \mathbf{u}}=\frac{\partial}{\partial \mathbf{u}}\left(V_{0} s \frac{\partial e}{\partial \mathbf{u}}\right)=V_{0} E \frac{\partial e}{\partial \mathbf{u}} \otimes \frac{\partial e}{\partial \mathbf{u}}+V_{0} s \frac{\partial^{2} e}{\partial \mathbf{u} \partial \mathbf{u}}=\mathbf{K}_{M}+\mathbf{K}_{G}\]

\hypertarget{truss-kinematics}{%
\subsection{6.2 Truss Kinematics}\label{truss-kinematics}}

\hypertarget{green-lagrange-strain}{%
\subsubsection{Green-Lagrange Strain}\label{green-lagrange-strain}}

\[v_{G L}=\frac{\Delta X}{L} \Delta \boldsymbol{u}_{x}+\frac{\Delta Y}{L} \Delta \boldsymbol{u}_{y}+\frac{\left(\Delta \boldsymbol{u}_{x}\right)^{2}}{2 L}+\frac{\left(\Delta \boldsymbol{u}_{y}\right)^{2}}{2 L}\]
