

$$E_{t}=\frac{d \sigma}{d \varepsilon}$$

$$s_r(x)=\int_{A} \mathbf{a}_{s}(y, z)^{T} \sigma_{m} d A=\left(\begin{array}{l}
N(x) \\
M_{z}(x) \\
M_{y}(x)
\end{array}\right)$$

$$\mathbf{k}_{s}=\frac{\partial s_r}{\partial e}=\int_{A} \mathbf{a}_{s}(y, z)^{T} \frac{d \sigma_{m}}{d \varepsilon_{m}} \frac{\partial \varepsilon_{m}}{\partial e} d A=\int_{A} \mathbf{a}_{s}(y, z)^{T} \frac{d \sigma_{m}}{d \varepsilon_{m}} \mathbf{a}_{s}(y, z) d A$$

$$s=\left(\begin{array}{l}
N \\
M
\end{array}\right)=\sum_{i=1}^{n I P}\left(\begin{array}{r}
1 \\
-y_{i}
\end{array}\right) \sigma_{i} b_{i} w_{i}$$

$$\mathbf{k}_{s}=\sum_{i=1}^{n I P}\left[\begin{array}{rr}
1 & -y_{i} \\
-y_{i} & y_{i}^{2}
\end{array}\right] E_{i} b_{i} w_{i}$$